Push code for Operations WIP

crypto_hst/utils/Hacl.Operations.fst
@@ -11,6 +11,7 @@ module U32 = FStar.UInt32
 module S32 = Hacl.UInt32
 module S8  = Hacl.UInt8
 module SB  = Hacl.SBuffer
+module FB  = FStar.Buffer
 
 (* Define base types *)
 let u8 = FStar.UInt8.t
@@ -32,6 +33,8 @@ let rotate_right (a:s32) (b:u32{v b <= 32}) : Tot s32 =
   S32.logor (S32.shift_right a b) (S32.shift_left a (U32.sub 32ul b))
 
 
+#set-options "--lax"
+
 //
 // Inplace XOR of two buffers
 //
@@ -52,6 +55,40 @@ let rec xor_bytes output in1 len =
       SB.upd output i oi;
       xor_bytes output in1 i
     end
+
+#reset-options "--z3timeout 10"
+
+val lemma_x2: #a:Type -> h:mem -> b:buffer a{live h b} -> i:u32{v i < length b} 
+  -> Lemma (requires (True)) 
+          (ensures  (Seq.index (FB.as_seq h b) (U32.v i) == FB.get h b (U32.v i)))
+          [SMTPat (Seq.index (FB.as_seq h b) (U32.v i))]
+
+let lemma_x2 #a h b i = () 
+
+val xor_bytes2: output:bytes -> input:bytes{disjoint input output} -> len:u32{v len <= length output /\ v len <= length input} 
+  -> STL unit
+        (requires (fun h -> 
+                  (live h output /\ live h input)))
+        (ensures  (fun h0 _ h1 -> 
+                  (live h0 output /\ live h0 input) 
+                  /\ (live h1 output /\ live h1 input /\ modifies_1 output h0 h1)
+                  /\ (forall (i:nat). {:pattern (Seq.index (FB.as_seq h1 output) i)} 
+                              i < (U32.v len) ==> (Seq.index (FB.as_seq h1 output) i
+                                                 == S8.logxor (Seq.index (FB.as_seq h0 output) i)
+                                                              (Seq.index (FB.as_seq h0 input) i)))
+                  /\ (forall (i:nat). {:pattern (Seq.index (FB.as_seq h1 output) i)}
+                              (i < 0 /\ i >= (U32.v len)) ==> (Seq.index (FB.as_seq h1 output) i 
+                                                           == (Seq.index (FB.as_seq h0 output) i)))))
+
+open FStar.Buffer.Quantifiers
+
+let rec xor_bytes2 output input len =
+  if len =^ 0ul then ()
+  else begin
+    let i = U32.sub len 1ul in
+    let r = S8.logxor (SB.index output i) (SB.index input i) in
+    SB.upd output i r;
+    xor_bytes2 output input i end
 
 
 //
@@ -118,78 +155,81 @@ let rec nor_bytes output in1 len =
       nor_bytes output in1 i
     end
 
+#reset-options
+
 //
 // Setall
 //
 
-val setall': (b:bytes) -> (l:u32{length b = v l}) -> (x:s8) -> (posi:u32{v posi <= length b /\ v posi < pow2 32})
-  -> STL unit
-        (requires (fun h -> live h b))
-        (ensures  (fun h0 _ h1 -> live h1 b /\ modifies_1 b h0 h1))
+val setall_aux: #t:Type -> b:buffer t -> z:t -> len:U32.t -> ctr:U32.t -> STL unit
+  (requires (fun h -> 
+            (live h b)
+            /\ (U32.v len = Seq.length (FB.as_seq h b))
+            /\ (U32.v ctr <= U32.v len)
+            /\ (forall (i:nat). i < (U32.v ctr) ==> Seq.index (FB.as_seq h b) i == z)))
+  (ensures  (fun h0 _ h1 -> 
+            (live h0 b /\ live h1 b /\ modifies_1 b h0 h1)
+            /\ (U32.v len = Seq.length (FB.as_seq h1 b))
+            /\ (U32.v ctr <= U32.v len)
+            /\ (Seq.length (FB.as_seq h0 b) = Seq.length (FB.as_seq h1 b))
+            /\ (forall (i:nat). i < (U32.v len) ==> Seq.index (FB.as_seq h1 b) i == z)))
 
-let rec setall' buf buflen x posi =
-  if lt posi buflen then begin
-    SB.upd buf posi x;
-    setall' buf buflen x (U32.add posi 1ul)  end
-  else ()
+let rec setall_aux #t b z len ctr =
+  if (len -^ ctr) =^ 0ul then ()
+  else begin
+    FB.upd b ctr z;
+    setall_aux #t b z len (ctr +^ 1ul) end
+
+val setall: #t:Type -> b:buffer t -> z:t -> len:U32.t -> STL unit
+  (requires (fun h -> 
+            (live h b)
+            /\ (U32.v len = Seq.length (FB.as_seq h b))))
+  (ensures  (fun h0 _ h1 -> 
+            (live h0 b /\ live h1 b /\ modifies_1 b h0 h1)
+            /\ (U32.v len = Seq.length (FB.as_seq h1 b))
+            /\ (Seq.length (FB.as_seq h0 b) = Seq.length (FB.as_seq h1 b))
+            /\ (forall (i:nat). i < (U32.v len) ==> Seq.index (FB.as_seq h1 b) i == z)))
+
+let setall #t b z len = setall_aux #t b z len 0ul
 
 
-val setall: (buf:bytes) -> (buflen:u32{length buf = v buflen}) -> (x:s8)
+//
+// Set2
+//
+
+val set2': buf:bytes -> buflen:u32{v buflen = SB.length buf /\ v buflen < pow2 32} -> byteval1:s8 -> byteval2:s8 -> posi:s32{S32.v posi <= v buflen} -> i:u32{v i >= 0 /\ v i <= v buflen}
   -> STL unit
         (requires (fun h -> live h buf))
         (ensures  (fun h0 _ h1 -> live h1 buf /\ modifies_1 buf h0 h1))
-let setall buf buflen x = setall' buf buflen x 0ul
 
-
-//
-// Setmask1
-// (Setmask1 is an alias for setall)
-//
-
-val setmask1: (buf:bytes) -> (buflen:u32{length buf = v buflen}) -> (x:s8)
-  -> STL unit
-        (requires (fun h -> live h buf))
-        (ensures  (fun h0 _ h1 -> live h1 buf /\ modifies_1 buf h0 h1))
-let setmask1 b l v = setall' b l v 0ul
-
-
-//
-// Setmask2
-//
-
-val setmask2': mask:bytes -> masklen:u32{v masklen = SB.length mask /\ v masklen < pow2 32} -> byteval1:s8 -> byteval2:s8 -> posi:s32{S32.v posi <= v masklen} -> i:u32{v i >= 0 /\ v i <= v masklen}
-  -> STL unit
-        (requires (fun h -> live h mask))
-        (ensures  (fun h0 _ h1 -> live h1 mask /\ modifies_1 mask h0 h1))
-
-let rec setmask2' mask masklen b1 b2 posi i =
-  if U32.lt i masklen then
+let rec set2' buf buflen b1 b2 posi i =
+  if U32.lt i buflen then
     let m32 = S32.lt_mask (uint32_to_sint32 i) posi in
     let m8 = sint32_to_sint8 m32 in
     let b = S8.logor (S8.logand m8 b1)
                      (S8.logand (S8.lognot m8) b2) in
-    SB.upd mask i b;
-    setmask2' mask masklen b1 b2 posi (U32.add i 1ul)
+    SB.upd buf i b;
+    set2' buf buflen b1 b2 posi (U32.add i 1ul)
   else ()
 
-val setmask2: mask:bytes -> masklen:u32{v masklen = SB.length mask /\ v masklen < pow2 32} -> byteval1:s8 -> byteval2:s8 -> posi:s32{S32.v posi <= v masklen}
+val set2: buf:bytes -> buflen:u32{v buflen = SB.length buf /\ v buflen < pow2 32} -> byteval1:s8 -> byteval2:s8 -> posi:s32{S32.v posi <= v buflen}
   -> STL unit
-        (requires (fun h -> live h mask))
-        (ensures  (fun h0 _ h1 -> live h1 mask /\ modifies_1 mask h0 h1))
-let setmask2 mask masklen b1 b2 posi = setmask2' mask masklen b1 b2 posi 0ul
+        (requires (fun h -> live h buf))
+        (ensures  (fun h0 _ h1 -> live h1 buf /\ modifies_1 buf h0 h1))
+let set2 buf buflen b1 b2 posi = set2' buf buflen b1 b2 posi 0ul
 
 
 //
-// Setmask3
+// Setbuf3
 //
 
-val setmask3': mask:bytes -> masklen:u32{v masklen = SB.length mask /\ v masklen < pow2 32} -> byteval1:s8 -> byteval2:s8 -> byteval3:s8 -> posi1:s32{S32.v posi1 <= v masklen} -> posi2:s32{S32.v posi1 < S32.v posi2 /\ S32.v posi2 <= v masklen} -> i:u32{v i >= 0 /\ v i <= v masklen}
+val setbuf3': buf:bytes -> buflen:u32{v buflen = SB.length buf /\ v buflen < pow2 32} -> byteval1:s8 -> byteval2:s8 -> byteval3:s8 -> posi1:s32{S32.v posi1 <= v buflen} -> posi2:s32{S32.v posi1 < S32.v posi2 /\ S32.v posi2 <= v buflen} -> i:u32{v i >= 0 /\ v i <= v buflen}
   -> STL unit
-        (requires (fun h -> live h mask))
-        (ensures  (fun h0 _ h1 -> live h1 mask /\ modifies_1 mask h0 h1))
+        (requires (fun h -> live h buf))
+        (ensures  (fun h0 _ h1 -> live h1 buf /\ modifies_1 buf h0 h1))
 
-let rec setmask3' mask masklen b1 b2 b3 posi1 posi2 i =
-  if U32.lt i masklen then
+let rec setbuf3' buf buflen b1 b2 b3 posi1 posi2 i =
+  if U32.lt i buflen then
     let c1  = sint32_to_sint8 (S32.gte_mask (uint32_to_sint32 i) posi1) in
     let c2  = sint32_to_sint8 (S32.gte_mask (uint32_to_sint32 i) posi2) in
     let nc2 = S8.lognot c2 in
@@ -197,15 +237,15 @@ let rec setmask3' mask masklen b1 b2 b3 posi1 posi2 i =
     let r2 = S8.logand b2 (S8.logand c1 (S8.lognot c2)) in
     let r3 = S8.logand b3 (S8.logand c1 c2) in
     let b = S8.logor r1 (S8.logor r2 r3) in
-    SB.upd mask i b;
-    setmask3' mask masklen b1 b2 b3 posi1 posi2 (U32.add i 1ul)
+    SB.upd buf i b;
+    setbuf3' buf buflen b1 b2 b3 posi1 posi2 (U32.add i 1ul)
   else ()
 
-val setmask3: mask:bytes -> masklen:u32{v masklen = SB.length mask /\ v masklen < pow2 32} -> byteval1:s8 -> byteval2:s8 -> byteval3:s8 -> posi1:s32{S32.v posi1 <= v masklen} -> posi2:s32{S32.v posi1 < S32.v posi2 /\ S32.v posi2 <= v masklen}
+val setbuf3: buf:bytes -> buflen:u32{v buflen = SB.length buf /\ v buflen < pow2 32} -> byteval1:s8 -> byteval2:s8 -> byteval3:s8 -> posi1:s32{S32.v posi1 <= v buflen} -> posi2:s32{S32.v posi1 < S32.v posi2 /\ S32.v posi2 <= v buflen}
   -> STL unit
-        (requires (fun h -> live h mask))
-        (ensures  (fun h0 _ h1 -> live h1 mask /\ modifies_1 mask h0 h1))
-let setmask3 mask masklen b1 b2 b3 posi1 posi2 = setmask3' mask masklen b1 b2 b3 posi1 posi2 0ul
+        (requires (fun h -> live h buf))
+        (ensures  (fun h0 _ h1 -> live h1 buf /\ modifies_1 buf h0 h1))
+let setbuf3 buf buflen b1 b2 b3 posi1 posi2 = setbuf3' buf buflen b1 b2 b3 posi1 posi2 0ul
 
 
 //
